\documentclass[11pt]{article}
\usepackage{amsmath}
\usepackage{amssymb}
\usepackage{amsfonts}
\usepackage[margin=1in]{geometry}

\begin{document}

\noindent Brandon Chen

\noindent MATH 395 HW 6

\noindent 6[2a, 4a], 7[3a, 36]

\noindent 7.48, 7.51, 7.40, 7.50

\begin{itemize}

	\item[6[2a,4a]]

		6.2) Suppose that 3 balls are chosen without replacement from an urn consisting of 5 white and 8 red balls. Let $X_i$ equal 1 if the $ith$ ball selected is white, and let it equal 0 otherwise. Give the joint probability mass function of 

		a) $X_1, X_2$
		
		Call $X_1 = X, X_2 = Y$

		$P(X=1, Y = 1) = \frac{5}{13} \frac{4}{12}$

		$P(X=1, Y = 0) = \frac{5}{13} \frac{8}{12}$

		$P(X=0, Y = 1) = \frac{8}{13} \frac{5}{12}$

		$P(X=0, Y = 0) = \frac{8}{13} \frac{7}{12}$

		6.4) Repeat problem 6.2 when the ball is selected and replaced before the next selection

		a) Call $X_1 = X, X_2 = Y$

		$P(X=1,Y = 1) = \frac{5}{13}\frac{5}{13}$

		$P(X=1,Y =0) = \frac{5}{13}\frac{8}{13}$

		$P(X=0, Y = 1) = \frac{8}{13} \frac{5}{13}$

		$P(X = 0, Y = 0) = \frac{8}{13} \frac{8}{13}$

	\item[6[3a, 36]]

		6.3) In problem 6.2, suppose that the white balls are numbered, and let $Y_i$ equal 1 if the $ith$ white ball is selected and 0 otherwise. Find hte joint probability mass function of 

		a) $Y_1, Y_2$

		3 balls are chosen, equally likely

		Want 1st white ball and 2nd white ball

		We picked 3, so probability of first is $\frac{3}{13}$

		Then the second white ball would have probability $\frac{2}{12}$

		$P(Y_1 = 1, Y_2 = 1) = \frac{3}{13} \frac{2}{12}$

		Similarly

		$P(Y_1 = 1, Y_2 = 0) = \frac{3}{13} \frac{10}{12}$

		$P(Y_1 = 0, Y_2 = 0) = \frac{10}{13} \frac{2}{12}$

		$P(Y_1 = 0, Y_2 = 0) = \frac{10}{13} \frac{9}{12}$

		6.36) In problem 6.3, calculate the conditional probability mass function of $Y_1$ given that 
		
		a) $Y_2 = 1$

		$P(Y_1 = 1 | Y_2 = 1) = \frac{\frac{3*2}{13*12}}{\frac{3}{13}} = \frac{1}{6}$

		$P(Y_1 = 0 | Y_2 = 1) = \frac{\frac{3*10}{13*12}}{\frac{3}{13}} = \frac{5}{6}$

		b) $Y_2 = 0$

		$P(Y_1 = 1| Y_2 = 0) = \frac{\frac{3*10}{13*12}}{\frac{10}{13}} = \frac{1}{4}$

		$P(Y_1 = 0 | Y_2 = 0) = \frac{\frac{10*9}{13*12}}{\frac{10}{13}} = \frac{3}{4}$

	\item[7.48]

		A fair die is successively rolled. Let $X,Y$ denote respectively, the number of rolls to obtain a 6 and a 5. Find

		a) $E[X]$

		$E[X] = \sum_{x=1}^{\infty} xP(X=x) = \sum_{x=1}^{\infty} x(\frac{5}{6}^{x-1} \frac{1}{6} = 6$

		$E[X] = 6$

		b) $E[X|Y = 1]$

		$E[X|Y = 1] = \sum_{x=1}^{\infty} xP(X=x | Y = 1) = \sum_{x=1}^{\infty} x\frac{5}{6}^{x-2} \frac{1}{6}$

		$=\frac{6}{5} \sum_{x=1} x\frac{5}{6}^{x-1} \frac{1}{6}$

		$=\frac{1}{5} \sum_{x=2} x\frac{5}{6}^{x-1}$

		$=\frac{-1}{5} + \frac{1}{5}*36$

		$=7$

		c) $E[X|Y = 5]$

		$=\sum_{x=1}^{\infty} xP(X = x, Y = 5)$

		$=\sum_{x=1}^{\infty} \frac{P(X = x, Y=5}{P(Y = 5)}$

		$P(Y = 5) = \frac{5}{6}^4 \frac{1}{6}$

		If $x \leq 4$, then $P(X = x, Y= 5) = (\frac{4}{6})^{x-1}\frac{1}{6} \frac{5}{6}^{4-x} \frac{1}{6}$

		If $x = 5$, then $P(X = x, Y =5) = \frac{4}{6}^{4} \frac{1}{6} \frac{5}{6}^{x-6} \frac{1}{6}$

		Then $E[X|Y = 5] = \frac{1}{(\frac{5}{6})^4(\frac{1}{6})} ( \sum_{x=1}^{4} x4^{x-1}5^{4-x}6^{-5} + \sum_{x=6}^{\infty} x4^45^{-x6}6^{-x})$

		$= \frac{3636}{625}$

	\item[7.51]

		The joint density of $X,Y$ is given by $f(x,y) = \frac{e^{-y}}{y}, \quad 0 < x < y, 0 < y < \infty$

		Compute $E[X^3 | Y=y]$

		$f_{X|Y}(x|y) = \frac{\frac{e^-y}{y}}{\int_0^y e^{-y}/y dx}, \quad 0 < x < y$

		$f_{X|Y}(x|y) = \frac{1}{y}, \quad 0 < x < y$

		$E[X^3 | Y = y] = \int_0^y x^3 \frac{1}{y} dx = \frac{y^3}{4}$



	\item[7.40]

		The joint density function of $X,Y$ is given by $f(x,y) = \frac{1}{y}e^{-(y+\frac{x}{y})}, \quad x > 0, y > 0$

		Find $E[X], E[Y]$, and show that $Cov(X,Y) = 1$

		$Cov(X,Y) = E[XY] - E[X]E[Y]$

		$f_Y(y) = e^{-y} \int_0^{\infty} \frac{1}{y} e^{-x/y} dx = e^{-y}$

		$E[Y] = \int_0^{\infty} e^{-y} = 1$

		Then $E[X] = E[E[X|Y]] = E[Y] = 1$

		$E[XY] = E[E[XY|Y] = E[Y E[X|Y]] = E[Y^2] = 2$

		Then $Cov(X,Y) = 2 - 1*1 = 1$

	\item[7.50]

		The joint density of $X,Y, f(x,y) = \frac{e^{\frac{-x}{y}} e^{-y}}{y}, \quad 0 < x < \infty, 0 < y < \infty$

		$f_{X|Y}(x|y) = \frac{e^{-x/y} e^{-y}/y}{\int_0^{\infty} e^{-x/y} e^{-y}/y dy}$

		$f_{X|Y}(x|y) = \frac{1}{y} e^{-x/y}, \quad 0< x< \infty$

		$E[X^2|Y = y] = \int_0^{\infty} x^2 \frac{1}{y} e^{-x/y} dx$

		$E[X^2 | Y=y] = 2y^2$
\end{itemize}
\end{document}
